Analysis complete.

theories/Analysis/AnalysisForwardSSA.v
@@ -15,10 +15,8 @@ Definition anni A (s:stmt) : Type :=
   end.
 
 Definition forwardF (sT:stmt) (Dom:stmt->Type) `{JoinSemiLattice (Dom sT)}
-           (forward:〔params〕 ->
-                    forall s (ST:subTerm s sT) (d:Dom sT),
+           (forward: forall s (ST:subTerm s sT) (d:Dom sT),
                       Dom sT)
-           (ZL:list params)
            (F:list (params * stmt)) (a:Dom sT)
            (ST:forall n s, get F n s -> subTerm (snd s) sT)
   : list (Dom sT).
@@ -27,35 +25,34 @@ Definition forwardF (sT:stmt) (Dom:stmt->Type) `{JoinSemiLattice (Dom sT)}
   destruct F as [|Zs F'].
   - eapply nil.
   - econstructor 2.
-    + refine (forward ZL (snd Zs) _ a).
+    + refine (forward (snd Zs) _ a).
       eapply (ST 0 Zs); eauto using get.
     + eapply (g F').
       eauto using get.
 Defined.
 
-Arguments forwardF [sT] [Dom] {H} {H0} forward ZL F a ST.
+Arguments forwardF [sT] [Dom] {H} {H0} forward F a ST.
 
 Fixpoint forwardF_length (sT:stmt) (Dom:stmt->Type) `{JoinSemiLattice (Dom sT)} forward
-           (ZL:list params)
            (F:list (params * stmt)) a
            (ST:forall n s, get F n s -> subTerm (snd s) sT) {struct F}
-  : length (forwardF forward ZL F a ST) = length F.
+  : length (forwardF forward F a ST) = length F.
 Proof.
   destruct F as [|Zs F']; simpl; eauto.
 Qed.
 
 Smpl Add
      match goal with
-     | [ |- context [ ❬@forwardF ?sT ?Dom ?H ?BSL ?f ?ZL ?F ?a ?ST❭ ] ] =>
-       rewrite (@forwardF_length sT Dom H BSL f ZL F a ST)
-     | [ H : context [ ❬@forwardF ?sT ?Dom ?H ?BSL ?f ?ZL ?F ?a ?ST❭ ] |- _ ] =>
-       rewrite (@forwardF_length sT Dom H BSL f ZL F a ST) in H
+     | [ |- context [ ❬@forwardF ?sT ?Dom ?H ?BSL ?f ?F ?a ?ST❭ ] ] =>
+       rewrite (@forwardF_length sT Dom H BSL f F a ST)
+     | [ H : context [ ❬@forwardF ?sT ?Dom ?H ?BSL ?f ?F ?a ?ST❭ ] |- _ ] =>
+       rewrite (@forwardF_length sT Dom H BSL f F a ST) in H
      end : len.
 
 Lemma forwardF_length_ass (sT:stmt) (Dom:stmt->Type) `{JoinSemiLattice (Dom sT)}
-      forward ZL F a ST k
+      forward F a ST k
   : length F = k
-    -> length (forwardF forward ZL F a ST) = k.
+    -> length (forwardF forward F a ST) = k.
 Proof.
   intros. rewrite forwardF_length, <- H1.
   repeat rewrite Nat.min_idempotent; eauto.
@@ -91,40 +88,58 @@ Definition option_extr A (o:option A) (x:A) :=
   | _ => x
   end.
 
+Lemma ZLIncl_ext sT st F t (ZL:list params)
+    (EQ:st = stmtFun F t) (ST:subTerm st sT)
+    (ZLIncl:list_union (of_list ⊝ ZL) [<=] occurVars sT)
+  : list_union (of_list ⊝ (fst ⊝ F ++ ZL)) [<=] occurVars sT.
+Proof.
+  subst.
+  rewrite List.map_app.
+  rewrite list_union_app. eapply union_incl_split; eauto.
+  pose proof (subTerm_occurVars ST). simpl in *.
+  rewrite <- H.
+  eapply incl_union_left. eapply list_union_incl; intros; eauto with cset.
+  inv_get. eapply incl_list_union. eapply map_get_1; eauto.
+  cset_tac.
+Qed.
+
 Fixpoint forward (sT:stmt) (Dom: stmt -> Type) `{JoinSemiLattice (Dom sT)}
          `{@LowerBounded (Dom sT) H}
            (ftransform :
-              forall sT, list params ->
-                    forall s, subTerm s sT -> Dom sT -> anni (Dom sT) s)
-           (ZL:list (params)) (st:stmt) (ST:subTerm st sT) (d:Dom sT) {struct st}
+              forall sT (ZL:list params) s,
+                subTerm s sT
+                -> list_union (of_list ⊝ ZL) [<=] occurVars sT
+                -> Dom sT -> anni (Dom sT) s)
+           (ZL:list (params)) (ZLIncl:list_union (of_list ⊝ ZL) [<=] occurVars sT)
+           (st:stmt) (ST:subTerm st sT) (d:Dom sT) {struct st}
   :  Dom sT.
   refine (
       match st as st' return st = st' -> Dom sT with
       | stmtLet x e s as st =>
         fun EQ =>
-          let d:Dom sT := anni_let (Dom sT) EQ (ftransform sT ZL st ST d) in
-        @forward sT Dom _ _ _ ftransform ZL s (subTerm_EQ_Let EQ ST) d
+          let d:Dom sT := anni_let (Dom sT) EQ (ftransform sT ZL st ST ZLIncl d) in
+        @forward sT Dom _ _ _ ftransform ZL ZLIncl s (subTerm_EQ_Let EQ ST) d
       | stmtIf x s t =>
         fun EQ =>
-          let an := anni_if EQ (ftransform sT ZL st ST d) in
+          let an := anni_if EQ (ftransform sT ZL st ST ZLIncl d) in
           match an with
           | (Some a, Some b) =>
-            let a' := @forward sT Dom _ H0 _ ftransform ZL s
+            let a' := @forward sT Dom _ H0 _ ftransform ZL ZLIncl s
                                (subTerm_EQ_If1 EQ ST) a in
-            let b' := @forward sT Dom _ H0 _ ftransform ZL t
+            let b' := @forward sT Dom _ H0 _ ftransform ZL ZLIncl t
                               (subTerm_EQ_If2 EQ ST) b in
             (join a' b')
             | (Some a, None) =>
-              @forward sT Dom _ H0 _ ftransform ZL s
+              @forward sT Dom _ H0 _ ftransform ZL ZLIncl s
                        (subTerm_EQ_If1 EQ ST) a
             | (None, Some b) =>
-              @forward sT Dom _ H0 _ ftransform ZL t
+              @forward sT Dom _ H0 _ ftransform ZL ZLIncl t
                        (subTerm_EQ_If2 EQ ST) b
             | (None, None) => bottom
           end
       | stmtApp f Y as st =>
         fun EQ =>
-          let d := anni_app (Dom sT) EQ (ftransform sT ZL st ST d) in
+          let d := anni_app (Dom sT) EQ (ftransform sT ZL st ST ZLIncl d) in
           d
 
     | stmtReturn x as st =>
@@ -134,10 +149,13 @@ Fixpoint forward (sT:stmt) (Dom: stmt -> Type) `{JoinSemiLattice (Dom sT)}
       fun EQ =>
         let ZL' := List.map fst F ++ ZL in
         let ant' :=
-            @forward sT Dom _ _ _ ftransform ZL' t (subTerm_EQ_Fun1 EQ ST)
+            @forward sT Dom _ _ _ ftransform ZL'
+                     (@ZLIncl_ext sT _ F t ZL EQ ST ZLIncl)
+                     t (subTerm_EQ_Fun1 EQ ST)
                                   d in
-        let anF' := forwardF (forward sT Dom _ _ _ ftransform) ZL' F d
-                            (subTerm_EQ_Fun2 EQ ST) in
+        let anF' := forwardF (forward sT Dom _ _ _ ftransform ZL'
+                                     (@ZLIncl_ext sT _ F t ZL EQ ST ZLIncl))
+                            F d (subTerm_EQ_Fun2 EQ ST) in
         fold_left join anF' ant'
       end eq_refl).
 Defined.
@@ -154,17 +172,15 @@ Proof.
 Qed.
 
 Lemma forwardF_get  (sT:stmt) (Dom:stmt->Type) `{JoinSemiLattice (Dom sT)}
-           (forward:〔params〕 ->
-                     forall s (ST:subTerm s sT) (d:Dom sT),
-                       Dom sT)
-           (ZL:list params)
-           (F:list (params * stmt)) a
-           (ST:forall n s, get F n s -> subTerm (snd s) sT) aa n
-           (GetBW:get (forwardF forward ZL F a ST) n aa)
-      :
-        { Zs : params * stmt & {GetF : get F n Zs &
-        { ST' : subTerm (snd Zs) sT | aa = forward ZL (snd Zs) ST' a
-        } } }.
+      (forward: forall s (ST:subTerm s sT) (d:Dom sT),
+          Dom sT)
+      (F:list (params * stmt)) a
+      (ST:forall n s, get F n s -> subTerm (snd s) sT) n aa
+           (GetBW:get (forwardF forward F a ST) n aa)
+  :
+    { Zs : params * stmt & {GetF : get F n Zs &
+                                   { ST' : subTerm (snd Zs) sT | aa = forward (snd Zs) ST' a
+    } } }.
 Proof.
   eapply get_getT in GetBW.
   general induction F; inv GetBW.
@@ -174,14 +190,13 @@ Proof.
 Qed.
 
 Lemma get_forwardF  (sT:stmt) (Dom:stmt->Type) `{JoinSemiLattice (Dom sT)}
-           (forward:〔params〕 ->
-                     forall s (ST:subTerm s sT) (d:Dom sT),
+           (forward: forall s (ST:subTerm s sT) (d:Dom sT),
                        Dom sT)
            (ZL:list params)
            (F:list (params * stmt)) (a:Dom sT)
            (ST:forall n s, get F n s -> subTerm (snd s) sT) n Zs
   :get F n Zs
-   -> { ST' | get (forwardF forward ZL F a ST) n (forward ZL (snd Zs) ST' a) }.
+   -> { ST' | get (forwardF forward F a ST) n (forward (snd Zs) ST' a) }.
 Proof.
   intros GetF.
   eapply get_getT in GetF.
@@ -193,8 +208,8 @@ Qed.
 
 Ltac inv_get_step_analysis_forward :=
   match goal with
-  | [ H: get (@forwardF ?sT ?Dom ?PO ?BSL ?f ?ZL ?F ?a ?ST) ?n ?x |- _ ]
-    => eapply (@forwardF_get sT Dom PO BSL f ZL F a ST x n) in H;
+  | [ H: get (@forwardF ?sT ?Dom ?PO ?BSL ?f ?F ?a ?ST) ?n ?x |- _ ]
+    => eapply (@forwardF_get sT Dom PO BSL f F a ST n x) in H;
       destruct H as [? [? [? ]]]
   end.
 
@@ -282,48 +297,47 @@ Proof.
   eapply bottom_least.
 Qed.
 
-Smpl Add 100 match goal with
-             | [ H : ?A === ?B |- _ ] => inv_if_ctor H A B
-             | [ H : poEq ?A ?B |- _ ] => inv_if_ctor H A B
-             | [ H : poLe ?A ?B |- _ ] => inv_if_ctor H A B
-             end : inv_trivial.
-
 Lemma forward_monotone (sT:stmt) (Dom : stmt -> Type) `{JoinSemiLattice (Dom sT)}
       `{@LowerBounded (Dom sT) H}
-      (f: forall sT, list params ->
-                forall s, subTerm s sT -> Dom sT -> anni (Dom sT) s)
-      (fMon:forall s (ST ST':subTerm s sT) ZL,
-          forall a b, a ⊑ b -> f sT ZL s ST a ⊑ f sT ZL s ST' b)
-  : forall (s : stmt) (ST ST':subTerm s sT) (ZL:list params),
-    forall (d d' : Dom sT), d ⊑ d' ->
-                           forward Dom f ZL ST d ⊑ forward Dom f ZL ST' d'.
+      (f: forall sT (ZL:list params),
+          forall s, subTerm s sT -> list_union (of_list ⊝ ZL) [<=] occurVars sT
+               -> Dom sT -> anni (Dom sT) s)
+      (fMon:forall s (ST ST':subTerm s sT) ZL
+          (ZLIncl ZLIncl':list_union (of_list ⊝ ZL) [<=] occurVars sT),
+          forall a b, a ⊑ b -> f sT ZL s ST ZLIncl a ⊑ f sT ZL s ST' ZLIncl' b)
+  : forall (s : stmt) (ST ST':subTerm s sT) (ZL:list params)
+      (ZLIncl ZLIncl':list_union (of_list ⊝ ZL) [<=] occurVars sT),
+    forall (d d' : Dom sT),
+      d ⊑ d'
+      -> forward Dom f ZL ZLIncl ST d ⊑ forward Dom f ZL ZLIncl' ST' d'.
 Proof with eauto using poLe_setTopAnn, poLe_getAnni.
   intros s.
-  sind s; destruct s; intros ST ST' ZL d d' LE_d; simpl forward;
+  sind s; destruct s; intros ST ST' ZL ZLIncl ZLIncl' d d' LE_d; simpl forward;
     simpl forward; repeat let_pair_case_eq; subst; eauto 10 using @ann_R;
       try now (econstructor; simpl; eauto using @ann_R).
   - eapply IH; eauto.
     (* Coq can't find the instantiation *)
     eapply (fMon (stmtLet x e s)); eauto.
-  - pose proof (fMon (stmtIf e s1 s2) ST ST' ZL _ _ LE_d).
+  - pose proof (fMon (stmtIf e s1 s2) ST ST' ZL ZLIncl ZLIncl' _ _ LE_d).
     pose proof (IH s1 ltac:(eauto) (subTerm_EQ_If1 eq_refl ST)
                                 (subTerm_EQ_If1 eq_refl ST') ZL) as LE1; eauto.
     pose proof (IH s2 ltac:(eauto) (subTerm_EQ_If2 eq_refl ST)
                                 (subTerm_EQ_If2 eq_refl ST') ZL) as LE2; eauto.
-    destruct (f sT ZL (stmtIf e s1 s2) ST d);
-      destruct (f sT ZL (stmtIf e s1 s2) ST' d'); simpl; invc H2;
+    destruct (f sT ZL (stmtIf e s1 s2) ST ZLIncl d);
+      destruct (f sT ZL (stmtIf e s1 s2) ST' ZLIncl' d'); simpl; invc H2;
         simpl snd in *; simpl fst in *; clear_trivial_eqs.
     repeat cases; subst; clear_trivial_eqs; simpl;
       try (specialize (LE1 _ _ H3));
       try (specialize (LE2 _ _ H4));
       eauto using bottom_least, join_struct, PIR2_bottom_least with len.
-    + rewrite LE1. eapply join_poLe.
-    + rewrite LE2. rewrite join_commutative. eapply join_poLe.
+    + rewrite LE1; eauto. eapply join_poLe; eauto.
+    + rewrite LE2; eauto. rewrite join_commutative. eapply join_poLe.
   - eapply (fMon (stmtApp l Y)); eauto.
   - simpl; fold_po.
     + eapply fold_left_join_struct; eauto.
       * eapply PIR2_get; eauto with len.
         intros; inv_get.
+
         eapply IH; eauto.
 Qed.
 
@@ -333,15 +347,17 @@ Instance makeForwardAnalysis (Dom:stmt -> Type)
          {PO:forall s, PartialOrder (Dom s)}
          (BSL:forall s, JoinSemiLattice (Dom s))
          (LB: forall s, @LowerBounded (Dom s) (PO s))
-         (f: forall sT, list params ->
-                   forall s, subTerm s sT -> Dom sT -> anni (Dom sT) s)
-         (fMon:forall sT s (ST ST':subTerm s sT) ZL,
-             forall a b, a ⊑ b -> f sT ZL s ST a ⊑ f sT ZL s ST' b)
+         (f: forall (sT : stmt) (ZL : 〔params〕) (s : stmt),
+             subTerm s sT ->
+             list_union (of_list ⊝ ZL) [<=] occurVars sT -> Dom sT -> anni (Dom sT) s)
+         (fMon:forall sT s (ST ST':subTerm s sT) ZL
+                 (ZLIncl ZLIncl':list_union (of_list ⊝ ZL) [<=] occurVars sT),
+             forall a b, a ⊑ b -> f sT ZL s ST ZLIncl a ⊑ f sT ZL s ST' ZLIncl' b)
          (Trm: forall s, Terminating (Dom s) poLt)
 
   : forall s, Iteration (Dom s) :=
   {
-    step := fun X : Dom s => forward Dom f nil (subTerm_refl _) X;
+    step := fun X : Dom s => forward Dom f nil (incl_empty _ _) (subTerm_refl _) X;
     initial_value := bottom
   }.
 Proof.
