theories/ValueOpts/ConstantPropagationAnalysis.v
@@ -1,4 +1,4 @@
-Require Import CSet Le CMap CMapDomain CMapPartialOrder CMapJoinSemiLattice.
+Require Import CSet Le CMap CMapDomain CMapPartialOrder CMapJoinSemiLattice CMapTerminating.
 
 Require Import Plus Util AllInRel CSet OptionR.
 Require Import Val Var Env IL Annotation Infra.Lattice DecSolve.
@@ -25,18 +25,7 @@ Qed.
 Smpl Add 100 match goal with
              | [ H : @poLe (withUnknown val) _ ?x ?y  |- _ ] =>
                eapply wua_poLe_inv in H; subst
-             | [ H : ~ ?a === ?a |- _ ] => exfalso; eapply H; reflexivity
-             | [ H : @poLe (withTop _) _ (wTA _) (wTA _) |- _ ] =>
-               eapply withTop_poLe_inv in H
-             | [ H : @poLe _ _ (wTA _) (wTA _) |- _ ] => invc H
-             | [ H : Known _ === Known _ |- _ ] => invc H
-             | [ H : withUnknown_eq _ _ |- _ ] =>
-               invc H
-             | [ H : withTop_le _ _ |- _ ] => invc H
-             | [ H : ?A === ?B |- _ ] => inv_if_ctor H A B
-             | [ H : poEq ?A ?B |- _ ] => inv_if_ctor H A B
              end : inv_trivial.
-
 
 
 Require Import MapNotations ListUpdateAt Subterm.
@@ -55,38 +44,6 @@ Fixpoint domupd_list (m:Dom) (A:list var) (B:list aval) :=
 
 Definition domenv (d:Dom) (x:var) : aval :=
   find x d.
-
-Definition constant_propagation_transform sT ZL st (ST:subTerm st sT)
-           (a:Dom)
-  : anni Dom st :=
-  match st as st', a return anni Dom st'  with
-  | stmtLet x (Operation e) s as st, d =>
-    let d' := domupd d x (op_eval (domenv d) e) in
-    d'
-  | stmtLet x (Call f Y) s as st, d =>
-    (* we assume renamed apart here, and dont zero x *)
-    domupd d x (Some Top)
-  | stmtIf e s t as st, d =>
-    if [op_eval (domenv d) e = Some (wTA val_true)] then
-      (Some d, None)
-    else if [op_eval (domenv d) e = Some (wTA val_false)] then
-           (None, Some d)
-         else if [op_eval (domenv d) e = None] then
-                (None, None)
-              else
-                (Some d, Some d)
-  | stmtApp f Y as st, d =>
-    let Z := nth (counted f) ZL (nil:list var) in
-    let Yc := List.map (op_eval (domenv d)) Y in
-    (* we assume renamed apart here, so it's ok to leave definitions
-       in d[X <-- Yc] that are /not/ defined at the point where f is defined *)
-    domupd_list d Z Yc
-  | stmtReturn e as st, d =>
-    d
-  | stmtFun F t as st, d =>
-    (* we assume renamed apart here, and dont zero Z *)
-    d
-  end.
 
 Instance eq_Refl
   : Reflexive (fun p p' : Dom * params => fst p ≣ fst p' /\ snd p = snd p').
@@ -127,6 +84,11 @@ Qed.
 
 Require Import Terminating OptionR.
 
+Smpl Add 100
+     match goal with
+     | [ H : @Equivalence.equiv val int_eq Equivalence_eq_int' _ _ |- _ ] =>
+       eapply int_eq_eq in H
+     end : inv_trivial.
 
 Lemma leMap_op_eval e a b
   : leMap a b
@@ -137,77 +99,24 @@ Proof.
   - unfold domenv.
     specialize (H n).
     destruct (find n a); eauto using fstNoneOrR.
-  - specialize (IHe _ _ H).
-    inv IHe; repeat cases;
-      simpl in *; clear_trivial_eqs; eauto using fstNoneOrR, @withTop_le.
-    econstructor. econstructor. congruence.
-    congruence.
+  - specialize (IHe _ _ H); repeat cases; eauto using fstNoneOrR, @withTop_le.
+    reflexivity.
   - specialize (IHe1 _ _ H).
     specialize (IHe2 _ _ H).
     inv IHe1; inv IHe2; repeat cases;
       simpl in *; clear_trivial_eqs;
         eauto using fstNoneOrR, withTop_le.
     + econstructor; econstructor. congruence.
-    + congruence.
 Qed.
 
-Ltac mlookup_eq_tac :=
-  match goal with
-  | [H : ?x === ?x' |- context[@find ?key ?OT ?FM ?elt ?x' (add ?x _ ?m) ] ]
-    => rewrite (@MapFacts.add_eq_o key OT FM _ elt m x x' _ H)
-  | [H : ?x === ?x', H' : context[@find ?key ?OT ?FM ?elt ?x' (add ?x _ ?m) ] |- _ ]
-    => rewrite (@MapFacts.add_eq_o key OT FM _ elt m x x' _ H) in H'
-  | [H : ?x === ?x' |- context[@find ?key ?OT ?FM ?elt ?x' (remove ?x ?m) ] ]
-    => rewrite (@MapFacts.remove_eq_o key OT FM _ elt m x x' H)
-  | [H : ?x === ?x', H' : context[@find ?key ?OT ?FM ?elt ?x' (remove ?x ?m) ]  |- _ ]
-    => rewrite (@MapFacts.remove_eq_o key OT FM _ elt m x x' H) in H'
-  end.
 
-Ltac mlookup_neq_tac :=
-   match goal with
-    | [ H : ~ ?x === ?x' |- context[@find ?key ?OT ?FM ?elt ?x' (add ?x _ ?m)] ]
-      => rewrite (@MapFacts.add_neq_o key OT FM _ elt m x x' _ H)
-    | [ H : ~ ?x === ?x', H' : context[@find ?key ?OT ?FM ?elt ?x' (add ?x _ ?m)] |- _ ]
-      => rewrite (@MapFacts.add_neq_o key OT FM _ elt m x x' _ H) in H'
-    | [ H : ~ ?x === ?x' |- context[@find ?key ?OT ?FM ?elt ?x' (remove ?x ?m)] ]
-      => rewrite (@MapFacts.remove_neq_o key OT FM _ elt m x x' H)
-    | [ H : ~ ?x === ?x', H' : context[@find ?key ?OT ?FM ?elt ?x' (remove ?x ?m)] |- _ ]
-      => rewrite (@MapFacts.remove_neq_o key OT FM _ elt m x x' H) in H'
-   end.
+Lemma poLe_option_None X `{PartialOrder X} (x:option X)
+  :  ⎣⎦ ⊑ x.
+Proof.
+  econstructor.
+Qed.
 
-
-Tactic Notation "smplmap" :=
-  repeat (repeat (subst || mlookup_eq_tac || mlookup_neq_tac)).
-
-
-Ltac lud :=
-  repeat (smplmap ||
-          match goal with
-          | [ x: _, x': _ |- context [@find ?key ?OT ?FM ?elt ?x' (add ?x _ ?m) ] ]
-      =>  match goal with
-          | [H' : x === x' |- _ ] => fail 1
-          | [H' : ~x === x' |- _ ] => fail 1
-          | [H' : x === x' -> False |- _ ] => fail 1
-          | [H' : x =/= x' |- _ ] => fail 1
-          | [ |- _ ] => decide(x === x')
-          end
-    | [ x: _, x': _, H : context[find ?x (add ?x' _ _)] |- _ ]
-      => match goal with
-          | [H' : x === x' |- _ ] => fail 1
-          | [H' : ~x === x' |- _ ] => fail 1
-          | [H' : x === x' -> False |- _ ] => fail 1
-          | [H' : x =/= x' |- _ ] => fail 1
-          | [ |- _ ] => decide(x === x')
-        end
-    | [ x: _, x': _ |- context [find ?x' (remove ?x _)] ]
-      => match goal with
-        | [H' : x === x' |- _ ] => fail 1
-        | [H' : ~x === x' |- _ ] => fail 1
-        | [H' : x === x' -> False |- _ ] => fail 1
-        | [H' : x =/= x' |- _ ] => fail 1
-        | [ |- _ ] => decide(x === x')
-        end
-          end).
+Hint Resolve poLe_option_None.
 
 Lemma domupd_le a b v v' x
   : leMap a b
@@ -216,13 +125,8 @@ Lemma domupd_le a b v v' x
 Proof.
   unfold leMap, domupd; intros.
   inv H0.
-  - repeat cases; simpl; clear_trivial_eqs.
-    lud; eauto using fstNoneOrR.
-    eapply H.
-    lud; eauto using fstNoneOrR.
-    eapply H.
-  - lud. econstructor; eauto.
-    eapply H.
+  - repeat cases; clear_trivial_eqs; mlud; eauto.
+  - mlud; eauto.
 Qed.
 
 Lemma domupd_list_le a b Z Y
@@ -245,6 +149,38 @@ Smpl Add match goal with
          | [ H : val_false = val_true |- _ ] => inv H
          end : inv_trivial.
 
+Definition constant_propagation_transform sT ZL st (ST:subTerm st sT)
+           (a:Dom)
+  : anni Dom st :=
+  match st as st', a return anni Dom st'  with
+  | stmtLet x (Operation e) s as st, d =>
+    let d' := domupd d x (op_eval (domenv d) e) in
+    d'
+  | stmtLet x (Call f Y) s as st, d =>
+    (* we assume renamed apart here, and dont zero x *)
+    domupd d x (Some Top)
+  | stmtIf e s t as st, d =>
+    if [op_eval (domenv d) e = Some (wTA val_true)] then
+      (Some d, None)
+    else if [op_eval (domenv d) e = Some (wTA val_false)] then
+           (None, Some d)
+         else if [op_eval (domenv d) e = None] then
+                (None, None)
+              else
+                (Some d, Some d)
+  | stmtApp f Y as st, d =>
+    let Z := nth (counted f) ZL (nil:list var) in
+    let Yc := List.map (op_eval (domenv d)) Y in
+    (* we assume renamed apart here, so it's ok to leave definitions
+       in d[X <-- Yc] that are /not/ defined at the point where f is defined *)
+    domupd_list d Z Yc
+  | stmtReturn e as st, d =>
+    d
+  | stmtFun F t as st, d =>
+    (* we assume renamed apart here, and dont zero Z *)
+    d
+  end.
+
 Lemma transf_mon
   : (forall (sT s : stmt) (ST ST' : subTerm s sT) (ZL : 〔params〕) (a b : Dom),
         a ⊑ b ->
@@ -256,15 +192,15 @@ Proof.
   - destruct e; eauto.
     + eapply domupd_le; eauto.
       eapply (leMap_op_eval e); eauto.
-    + hnf; intros. lud; eauto.
+    + hnf; intros. mlud; eauto.
   - exploit (leMap_op_eval e); eauto.
     repeat cases; split; eauto using @fstNoneOrR;
       try congruence; rewrite COND in *; try rewrite COND0 in *;
         simpl in *;
         clear_trivial_eqs.
-    inv H0; try congruence. inv H3. clear_trivial_eqs.
+    inv H0; try congruence. clear_trivial_eqs.
     rewrite <- H1 in *. isabsurd.
-    inv H0; try congruence. inv H3. clear_trivial_eqs.
+    inv H0; try congruence. clear_trivial_eqs.
     rewrite <- H1 in *. isabsurd.
     inv H0; try congruence. inv H0; congruence.
   - destruct (get_dec ZL l); dcr.
@@ -274,7 +210,122 @@ Proof.
     + rewrite not_get_nth_default; eauto.
 Qed.
 
+Definition DDom (sT:stmt) := { m : Map [var, withTop val] | domain m ⊆ occurVars sT}.
+
+Smpl Add 100
+     match goal with
+     | [ H : (_, _) = (_,_) |- _ ] => invc H
+     end : inv_trivial.
+
+Lemma domain_domupd_incl m x v
+  : domain (domupd m x v) ⊆ {x; domain m}.
+Proof.
+  unfold domupd; cases.
+  - rewrite domain_add. reflexivity.
+  - rewrite domain_remove. cset_tac.
+Qed.
+
+Lemma domain_domupd_list_incl m x v
+  : domain (domupd_list m x v) ⊆ of_list x ∪ domain m.
+Proof.
+  general induction x; destruct v; simpl.
+  - cset_tac.
+  - cset_tac.
+  - cset_tac.
+  - rewrite domain_domupd_incl.
+    rewrite IHx; eauto. cset_tac.
+Qed.
+
+Definition cp_trans_dep sT (ZL:list params) st (ST:subTerm st sT)
+           (ZLIncl: list_union (of_list ⊝ ZL) ⊆ occurVars sT) (a:DDom sT)
+  : anni (DDom sT) st.
+Proof.
+  set (res:=(@constant_propagation_transform sT ZL st ST (proj1_sig a))).
+  pose proof (subTerm_occurVars ST) as Incl. destruct a; simpl in *.
+  destruct st; simpl in *.
+  - destruct e.
+    + refine (exist _ res _); subst res.
+      rewrite domain_domupd_incl.
+      revert s Incl; cset_tac.
+    + refine (exist _ res _); subst res.
+      rewrite domain_add.
+      revert s Incl; cset_tac.
+  - refine (match res return
+                  (res = if [op_eval (domenv x) e = ⎣ wTA val_true ⎦] then (⎣ x ⎦, ⎣⎦) else if [op_eval (domenv x) e = ⎣ wTA val_false ⎦] then (⎣⎦, ⎣ x ⎦) else if [op_eval (domenv x) e = ⎣⎦] then (⎣⎦, ⎣⎦) else (⎣ x ⎦, ⎣ x ⎦)) -> ؟ (DDom sT) * ؟ (DDom sT)
+            with
+            | (Some x, Some y) => fun EQ => (Some (exist _ x _) , Some (exist _ y _))
+            | (Some x, None) => fun EQ => (Some (exist _ x _) ,None)
+            | (None, Some y) => fun EQ => (None, Some (exist _ y _))
+            | (None, None) => fun EQ => (None,None)
+            end eq_refl);
+      repeat cases in EQ; clear_trivial_eqs; eauto.
+  - refine (exist _ res _); subst res.
+    destruct (get_dec ZL l); dcr.
+    + erewrite get_nth; eauto.
+      rewrite domain_domupd_list_incl.
+      eapply union_incl_split; eauto.
+      rewrite <- ZLIncl.
+      eapply incl_list_union; eauto using map_get_1.
+    + rewrite not_get_nth_default; eauto.
+  - refine (exist _ res _); subst res. eauto.
+  - refine (exist _ res _); subst res. eauto.
+Defined.
+
+
+Lemma transf_mon_dep
+  : (forall (sT s : stmt) (ST ST' : subTerm s sT) (ZL : 〔params〕)
+       (ZLIncl ZLIncl': list_union (of_list ⊝ ZL) ⊆ occurVars sT) (a b : DDom sT),
+        a ⊑ b ->
+        cp_trans_dep ZL ST ZLIncl a ⊑ cp_trans_dep ZL ST' ZLIncl' b).
+Proof.
+  intros. destruct a as [a aBound], b as [b bBound]; simpl in H.
+  pose proof (@transf_mon sT s ST ST' ZL a b H) as LE.
+  destruct s; clear_trivial_eqs; simpl in *; eauto.
+  - destruct e; simpl; eauto.
+  - repeat (cases in LE; simpl in *); dcr;
+            clear_trivial_eqs; eauto using fstNoneOrR.
+Qed.
+
+Instance map_sig_semilattice_bound X `{OrderedType X} Y `{JoinSemiLattice Y}  U
+  : JoinSemiLattice ({ m : Map [X, Y] | domain m ⊆ U}) := {
+  join x y := exist _ (join (proj1_sig x) (proj1_sig y)) _
+}.
+Proof.
+  - destruct x,y; simpl.
+    unfold joinMap. rewrite domain_join. cset_tac.
+  - hnf; intros [a ?]. simpl. eapply joinDom_idem.
+  - hnf; intros [a ?] [b ?]. eapply joinDom_sym.
+  - hnf; intros [a ?] [b ?] [c ?]. eapply joinDom_assoc.
+  - hnf; intros [a ?] [b ?]; simpl. eapply joinDom_exp.
+  - simpl. unfold Proper, respectful; intros. destruct x,y,x0,y0; simpl in * |- *.
+    rewrite H2, H3. reflexivity.
+  - simpl. unfold Proper, respectful; intros. destruct x,y,x0,y0; simpl in * |- *.
+    rewrite H3, H2. reflexivity.
+Defined.
+
+Instance map_sig_lower_bounded X `{OrderedType X} Y `{JoinSemiLattice Y} U
+  : LowerBounded { m : Map [X, Y] | domain m ⊆ U} :=
+  {
+    bottom := exist _ (empty _) (incl_empty _ _)
+  }.
+Proof.
+  intros [a b]; simpl.
+  eapply empty_bottom; eauto.
+Defined.
+
+Instance
+  : Terminating (withTop val) poLt.
+Proof.
+  hnf; intros.
+  destruct x.
+  - econstructor; intros. inv H. inv H0. inv H. exfalso; eauto.
+  - econstructor; intros. inv H. inv H0.
+    + eapply int_eq_eq in H3. subst.
+      exfalso. eapply H1. eauto.
+    + econstructor; intros.
+      inv H2. inv H3. inv H2. exfalso; eauto.
+Qed.
 
 Definition constant_propagation_analysis :=
-  makeForwardAnalysis _ _ _ constant_propagation_transform transf_mon
-                      (fun _ => terminating_Dom).
+  makeForwardAnalysis DDom _ _ cp_trans_dep transf_mon_dep
+                      (fun s => (@terminating_Dom var _ _ _ (occurVars s) _)).
